WIP: started adding typing rules

theories/prob_eff_lang/probblaze/typing/types.v
@@ -1,6 +1,6 @@
 From Autosubst Require Import Autosubst.
 From stdpp Require Export strings gmultiset gmap stringmap.
-From clutch.prob_eff_lang.probblaze Require Import syntax.
+From clutch.prob_eff_lang.probblaze Require Import syntax notation.
 From iris.prelude Require Import prelude.
 
 
@@ -43,6 +43,7 @@ Section syntax.
   | TUnit : type
   | TBool : type
   | TInt  : type
+  | TNat  : type
 
   (* Reference type. *)
   | TRef : type → type
@@ -118,6 +119,98 @@ Section syntax.
   Global Instance SubstLemmas_mode : SubstLemmas vmode. derive. Defined.
   
 End syntax.
+
+
+
+Declare Scope FType_scope.
+Delimit Scope FType_scope with ty.
+Bind Scope FType_scope with type.
+Notation "()" := TUnit : FType_scope.
+Notation "⊥" := TBot : FType_scope.
+Notation "⊤" := TTop : FType_scope.
+Notation "'ℤ'" := TInt : FType_scope.
+Notation "'ℕ'" := TNat : FType_scope.
+Notation "'𝔹'" := TBool : FType_scope.
+
+(* Notation "# x" := (TVar x) (at level 100, x at next level): FType_scope. *)
+Infix "*" := TProd : FType_scope.
+Notation "(*)" := TProd (only parsing) : FType_scope.
+Infix "+" := TSum : FType_scope.
+Notation "(+)" := TSum (only parsing) : FType_scope.
+(* TODO: add arrow notation *)
+Notation "α '-{' ρ '}-∘' β" := (TArrow α%ty ρ β%ty)
+                                 (at level 100, ρ, β at level 200) : FType_scope.
+Notation "α -∘ β" := (TArrow α%ty RNil β%ty)
+                       (at level 100, β at level 200) : FType_scope.
+Notation "α '-{' ρ '}->' β" := (TBang MS (TArrow α%ty ρ β%ty))
+                                 (at level 100, ρ, β at level 200) : FType_scope.
+Notation "α ⇾ β" := (TBang MS (TArrow α%ty RNil β%ty))
+                       (at level 100, β at level 200) : FType_scope.
+Notation "μ: τ" :=
+  (TRec τ%ty)
+  (at level 100, τ at level 200) : FType_scope.
+Notation "∀T: τ" :=
+  (TForallT τ%ty)
+    (at level 100, τ at level 200) : FType_scope.
+Notation "∀R: τ" :=
+  (TForallR τ%ty)
+    (at level 100, τ at level 200) : FType_scope.
+Notation "∀M: τ" :=
+  (TForallM τ%ty)
+  (at level 100, τ at level 200) : FType_scope.
+Notation "∃: τ" :=
+  (TExists τ%ty)
+  (at level 100, τ at level 200) : FType_scope.
+Notation "'ref' τ" := (TRef τ%ty) (at level 10, τ at next level, right associativity): FType_scope.
+Notation "![ m ] τ" := (TBang m τ%ty) (at level 10, τ at next level, right associativity): FType_scope.
+(* Notation "! τ" := (TBang MS τ%ty) (at level 10, τ at next level, right associativity): FType_scope. *)
+
+
+Section ctx.
+
+  (* A ctx is a multiset of key-value pairs restricting the value to be the same for each instance of the key *)
+  Definition ctx := gmap string (type * nat).
+
+  (* insert sets the multiplicity to 1 *)
+  Definition ctx_insert (x : string) (t : type) (Γ : ctx) : ctx := <[ x := (t, 1) ]> Γ.
+
+  (* duplicate a variable in the ctx *)
+  Definition ctx_contraction (x : string) (Γ : ctx) : ctx :=
+    match Γ !! x with
+    | Some (t, n) => <[ x := (t, S n) ]> Γ
+    | None => Γ
+    end. 
+
+  Definition ctx_remove (x : string) (Γ : ctx) : ctx :=
+  match Γ !! x with
+  | Some (t, S n) => 
+      if decide (n = 0) 
+      then delete x Γ 
+      else <[ x := (t, n) ]> Γ
+  (* Not strictly necessary since we remove an instance of 0 multiplicity *)
+  | Some (t, 0) => delete x Γ
+  | _ => Γ
+  end.
+
+  Definition ctx_lookup (x : string) (Γ : ctx) : option type := fmap fst (Γ !! x).
+
+  (* We shouldn't merge to ctx where (x : t) ∈ Γ1 and (x : t') ∈ Γ2 s.t. t ≠ t'  *)
+  Definition merge_aux : option (type * nat) → option (type * nat) → option (type * nat) :=
+    λ a b,
+      match a, b with
+      | x, None
+      | None, x => x
+      | Some (t, n), Some (t', n') => Some (t, n + n')
+      end. 
+  Definition ctx_append (Γ1 Γ2 : ctx) : ctx := gmap_merge _ _ _ merge_aux Γ1 Γ2.
+
+End ctx.
+
+Notation "'<[' x ':=c' t ']>' Γ" := (ctx_insert x t Γ).
+Notation "Γ '!!c' x" := (ctx_lookup x Γ) (at level 100, x at next level).
+Notation "'<[' x ':=c + ]>' Γ" := (ctx_contraction x Γ).
+Notation "'<[' x ':=c - ]>' Γ" := (ctx_remove x Γ).
+Notation "Γ1 ';;' Γ2" := (ctx_append Γ1 Γ2) (at level 100).
 
 (** * Weakening Relation. *)
 
@@ -223,7 +316,7 @@ Module le.
     _row D false ρ ρ' →
     _row D b (RCons σ ρ) (RCons σ' ρ')
   (* Notice js is atmost the singleton {i} *)
-  | RErase_le D s ρ ss js :
+  | RErase_le (D : disj_ctx) s ρ ss js :
     D !! s = Some (ss, js) →
     conc_sigs ρ ⊆ ss →
     abst_sigs ρ ⊆ js →
@@ -281,6 +374,8 @@ Module le.
           
   | TBangBool_le D m : _type D TBool (TBang m TBool)
   | TBangUnit_le D m : _type D TUnit (TBang m TUnit)
+  | TBangInt_le D m : _type D TInt (TBang m TInt)
+  | TBangNat_le D m : _type D TNat (TBang m TNat)
   | TBangTop_le D m : _type D TTop (TBang m TTop)
   | TBangRef_le D m α : _type D (TRef α) (TBang m (TRef α))
                               (* TODO: unsure if this is sound. *)
@@ -299,9 +394,257 @@ Module le.
   | TBangTForallRComm1_le D m α : _type D (TBang m (TForallR α)) (TForallR (TBang m α))
   | TBangTForallRComm2_le D m α : _type D (TForallR (TBang m α)) (TBang m (TForallR α)).
 
-  .
-         
-      
+  Definition MultiT (τ : type) : Prop := _type ∅ τ (![MS] τ).
+
+  Definition OnceR (ρ : row) : Prop := ∃ b, _row ∅ b (RFlip MS ρ) ρ. 
+
+  (* Lifting Multi from types to ctx *)
+  Definition MultiC (Γ : ctx) : Prop := Forall MultiT (fmap fst (fmap snd (map_to_list Γ))). 
+
+  Inductive _mode_type : vmode → type → Prop :=
+  | OS_le τ : _mode_type OS τ
+  | MS_le τ : MultiT τ → _mode_type MS τ.
+
+  Inductive _mode_ctx : vmode → ctx → Prop :=
+  | NilM_le m : _mode_ctx m ∅
+  | ConsM_le m x τ Γ : _mode_type m τ → _mode_ctx m Γ → _mode_ctx m (<[ x :=c τ ]> Γ).
+
+  Inductive _row_type : row → type → Prop :=
+  | Once_le ρ τ : OnceR ρ → _row_type ρ τ
+  | Multi_le ρ τ : MultiT τ → _row_type ρ τ.
+
+  Inductive _row_ctx : row → ctx → Prop :=
+  | NilR_le ρ : _row_ctx ρ ∅
+  | ConsR_le ρ x τ Γ : _row_type ρ τ → _row_ctx ρ Γ → _row_ctx ρ (<[ x :=c τ ]> Γ).
+  
+End le.
+
+Notation "D ⊢ α ≤T α'" := (le._type D α α')
+  (at level 74, α, α' at next level).
+Notation "D ⊢ ρ ≤R ρ' @ b" := (le._row D b ρ ρ')
+  (at level 74, ρ, ρ', b at next level).
+Notation "D ⊢ σ ≤S σ'" := (le._eff_sig D σ σ')
+  (at level 74, σ, σ' at next level).
+Notation "⊢ m ≤M m'" := (le._mode m m')
+  (at level 74, m, m' at next level).
+Notation "m 'm⪯T' τ" := (le._mode_type m τ) (at level 74, τ at next level).  
+Notation "m 'm⪯C' Γ" := (le._mode_ctx m Γ) (at level 74, Γ at next level).
+Notation "ρ 'R⪯T' τ" := (le._row_type ρ τ) (at level 74, τ at next level).
+Notation "ρ 'R⪯C' Γ" := (le._row_ctx ρ Γ) (at level 74, Γ at next level).
+
+(** Which types are unboxed -- we can only do CAS on locations which hold unboxed types *)
+Inductive UnboxedType : type → Prop :=
+  | UnboxedTUnit : UnboxedType TUnit
+  | UnboxedTNat : UnboxedType TNat
+  | UnboxedTInt : UnboxedType TInt
+  | UnboxedTBool : UnboxedType TBool
+  | UnboxedTRef τ : UnboxedType (TRef τ).
+
+(** Types which support direct equality test (which coincides with ctx equiv).
+    This is an auxiliary notion. *)
+Inductive EqType : type → Prop :=
+  | EqTUnit : EqType TUnit
+  | EqTNat : EqType TNat
+  | EqTInt : EqType TInt
+  | EqTBool : EqType TBool
+  | EqTProd τ τ' : EqType τ → EqType τ' → EqType (TProd τ τ')
+  | EqSum τ τ' : EqType τ → EqType τ' → EqType (TSum τ τ')
+  (* | EQRef τ : EqType (Tref τ) *)
+.
+
+Lemma unboxed_type_ref_or_eqtype τ :
+  UnboxedType τ → (EqType τ ∨ (∃ τ', τ = TRef τ') ∨ τ = TTape).
+Proof. inversion 1; first [ left; by econstructor | right; naive_solver ]. Qed.
+
+Definition binop_int_res_type (op : bin_op) : option type :=
+  match op with
+  | PlusOp | MinusOp | MultOp | QuotOp | RemOp => Some TInt
+  | AndOp | OrOp | XorOp => None
+  | ShiftLOp | ShiftROp => Some TInt
+  | LeOp | LtOp | EqOp => Some TBool
+  | OffsetOp => Some TInt
+  end.
+Definition binop_bool_res_type (op : bin_op) : option type :=
+  match op with
+  | PlusOp | MinusOp | MultOp | QuotOp | RemOp => None
+  | AndOp | OrOp | XorOp => Some TBool
+  | ShiftLOp | ShiftROp => None
+  | LeOp | LtOp => None
+  | EqOp => Some TBool
+  | OffsetOp => None
+  end.
+Definition unop_int_res_type (op : un_op) : option type :=
+  match op with
+  | NegOp => None
+  | MinusUnOp => Some TInt
+  end.
+Definition unop_bool_res_type (op : un_op) : option type :=
+  match op with
+  | NegOp => Some TBool
+  | MinusUnOp => None
+  end.
+
+(** Operation lifts *)
+Global Instance insert_binder (A : Type): Insert binder A (stringmap A) :=
+  binder_insert.
+
+
+Module vars.
+
+  Fixpoint _eff_sig (f : type → gset eff_name) (σ : eff_sig) : gset eff_name :=
+    match σ with
+    | SSig s α β => {[ s ]} ∪ (f α) ∪ (f β)
+    | SFlip _ σ => _eff_sig f σ
+    end.
+
+  Fixpoint _row_pre (f : type → gset eff_name) (ρ : row) : gset eff_name :=
+    match ρ with
+    | RNil
+    | RVar _ => ∅
+    | RFlip _ ρ
+    | RRec ρ => _row_pre f ρ
+    | RCons σ ρ => _eff_sig f σ ∪ _row_pre f ρ
+    end.
+
+  Fixpoint _ty (α : type) : gset eff_name :=
+    match α with
+    | TTop
+    | TBot
+    | TUnit
+    | TBool
+    | TInt
+    | TNat
+    | TTape
+    | TVar _ =>
+        (∅ : gset eff_name)
+    | TProd α β
+    | TSum α β =>
+        (_ty α) ∪ (_ty β)
+    | TRef α
+    | TRec α
+    | TBang _ α
+    | TExists α
+    | TForallT α
+    | TForallR α
+    | TForallM α =>
+        (_ty α)
+    | TArrow α ρ β =>
+        (_ty α) ∪ (_row_pre _ty ρ) ∪ (_ty β)
+    end.
+  
+  Definition _row : row → gset eff_name :=
+    _row_pre _ty.
+  
+  Definition _ctx (Γ : ctx) : gset eff_name :=
+    ⋃ ((λ '(_, (α, _)), _ty α) <$> (map_to_list Γ)).
+
+  (* REMARK : unsure if we need to make the check that s is free in dom Γ *)
+  (* since this is probably dependent on the implementation of subst *)
+  (* The assertion [fresh s Γ ρ α] holds if the string [s] is free in
+     [ρ], [α], and [Γ], when seen as an effect name, and it must also not
+     appear in the domain of [Γ]. *)
+  Definition _fresh s Γ ρ α :=
+    s ∉ vars._ctx Γ ∧
+    s ∉ vars._row ρ ∧
+    s ∉ vars._ty α.
+
+End vars.
+
+
+Reserved Notation "Δ '.|' Γ1 '⊢ₜ' e ':' ρ ':' τ '⊣' Γ2"
+  (at level 74, Γ1, e, ρ, τ, Γ2 at next level).
+Reserved Notation "'⊢ᵥ' v ':' τ"  (at level 20, v, τ at next level).
+
+(* From clutch.prob_eff_lang.probblaze Require Import notation. *)
+
+Inductive typed :
+  stringmap unit → ctx → expr → row → type → ctx → Prop :=
+
+| Var_typed Δ Γ x τ :
+  ctx_lookup x Γ = Some τ →
+  Δ .| Γ ⊢ₜ Var x : RNil : τ ⊣ (ctx_remove x Γ)
+
+| Val_typed Δ Γ v ρ τ :
+  ⊢ᵥ v : τ →
+  Δ .| Γ ⊢ₜ Val v : ρ : τ ⊣ Γ
+
+| Pair_typed Δ Γ1 Γ2 Γ3 e1 e2 ρ τ1 τ2 :
+  Δ .| Γ1 ⊢ₜ e1 : ρ : τ1 ⊣ Γ2 →
+                    Δ .| Γ2 ⊢ₜ e2 : ρ : τ2 ⊣ Γ3 →
+                                       Δ .| Γ1 ⊢ₜ Pair e1 e2 : ρ : τ1 * τ2 ⊣ Γ3
+
+| Fst_typed Δ Γ1 e ρ τ1 τ2 Γ2 :
+  Δ .| Γ1 ⊢ₜ e : ρ : τ1 * τ2  ⊣ Γ2 →
+                    Δ .| Γ1 ⊢ₜ Fst e : ρ : τ1 ⊣ Γ2
+| Snd_typed Δ Γ1 e ρ τ1 τ2 Γ2 :
+  Δ .| Γ1 ⊢ₜ e : ρ : τ1 * τ2  ⊣ Γ2 →
+                    Δ .| Γ1 ⊢ₜ Snd e : ρ : τ2 ⊣ Γ2
+
+| InjL_typed Δ Γ1 e ρ τ1 τ2 Γ2 :
+  Δ .| Γ1 ⊢ₜ e : ρ : τ1 ⊣ Γ2 →
+                    Δ .| Γ1 ⊢ₜ InjL e : ρ : τ1 + τ2 ⊣ Γ2
+| InjR_typed Δ Γ1 e ρ τ1 τ2 Γ2 :
+  Δ .| Γ1 ⊢ₜ e : ρ : τ2 ⊣ Γ2 →
+                    Δ .| Γ1 ⊢ₜ InjR e : ρ : τ1 + τ2 ⊣ Γ2
+| Case_typed Δ Γ1 Γ2 Γ3 e0 e1 e2 ρ τ1 τ2 τ3 :
+  Δ .| Γ1 ⊢ₜ e0 : ρ : τ1 + τ2 ⊣ Γ2 →
+                     Δ .| Γ2 ⊢ₜ e1 : ρ : τ1 -{ ρ }-∘ τ3 ⊣ Γ3 →
+                                        Δ .| Γ2 ⊢ₜ e2 : ρ : τ2 -{ ρ }-∘ τ3 ⊣ Γ3 →
+                                                           Δ .| Γ1 ⊢ₜ Case e0 e1 e2 : ρ : τ3 ⊣ Γ3
+
+| If_typed Δ Γ1 Γ2 Γ3 e0 e1 e2 ρ τ :
+  Δ .| Γ1 ⊢ₜ e0 : ρ : 𝔹 ⊣ Γ2 →
+                     Δ .| Γ2 ⊢ₜ e1 : ρ : τ ⊣ Γ3 →
+                                        Δ .| Γ2 ⊢ₜ e2 : ρ : τ ⊣ Γ3 →
+                                                           Δ .| Γ1 ⊢ₜ If e0 e1 e2 : ρ : τ ⊣ Γ3
+(* TODO: consider other rules for affine function types *)
+| Rec_typed Δ Γ f x e ρ τ κ :
+  Δ .| <[ f :=c (τ -{ ρ }-> κ)%ty ]> <[ x :=c τ ]> Γ ⊢ₜ e : ρ : κ ⊣ ∅ →
+                                                             Δ .| Γ ⊢ₜ Rec f x e : RNil : τ -{ ρ }-> κ ⊣ ∅
+(* TODO: generalize according to Fig. 5 in Affect *)
+| App_typed Δ Γ1 Γ2 Γ3 e1 e2 ρ τ κ :
+  Δ .| Γ1 ⊢ₜ e2 : ρ : τ ⊣ Γ2 →
+                     Δ .| Γ2 ⊢ₜ e1 : ρ : τ -{ ρ }-∘ κ ⊣ Γ3 →
+                                        Δ .| Γ1 ⊢ₜ App e1 e2 : ρ : κ ⊣ Γ3
+
+| TAlloc Δ Γ1 e ρ τ Γ2 : Δ .| Γ1 ⊢ₜ e : ρ : τ ⊣ Γ2  → Δ .| Γ1 ⊢ₜ AllocN (Val $ LitV $ LitInt 1) e : ρ : ref τ ⊣ Γ2
+| TLoad Δ Γ1 e ρ τ Γ2 : Δ .| Γ1 ⊢ₜ e : ρ : ref τ ⊣ Γ2 → Δ .| Γ1 ⊢ₜ Load e : ρ : τ ⊣ Γ2
+| TStore Δ Γ1 Γ2 Γ3 e e' ρ τ :
+  Δ .| Γ1 ⊢ₜ e' : ρ : τ ⊣ Γ2 → 
+                     Δ .| Γ2 ⊢ₜ e : ρ : ref τ ⊣ Γ3 → 
+                                       Δ .| Γ1 ⊢ₜ Store e e' : ρ : () ⊣ Γ3
+| TAllocTape Δ Γ1 e ρ Γ2 : Δ .| Γ1 ⊢ₜ e : ρ : ℕ ⊣ Γ2 →  Δ .| Γ1 ⊢ₜ AllocTape e : ρ : TTape ⊣ Γ2
+| TRand Δ Γ1 Γ2 Γ3 e1 e2 ρ : Δ .| Γ2 ⊢ₜ e1 : ρ : ℕ ⊣ Γ3 → Δ .| Γ1 ⊢ₜ e2 : ρ : TTape ⊣ Γ2 → Δ .| Γ1 ⊢ₜ Rand e1 e2 : ρ : ℕ ⊣ Γ3
+| TRandU Δ Γ1 Γ2 Γ3 e1 e2 ρ : Δ .| Γ2 ⊢ₜ e1 : ρ : ℕ ⊣ Γ3 → Δ .| Γ1 ⊢ₜ e2 : ρ : () ⊣ Γ2 → Δ .| Γ1 ⊢ₜ Rand e1 e2 : ρ : ℕ ⊣ Γ3
+(* TODO: add to subsumption rules
+   | Subsume_int_nat Γ e : Γ ⊢ₜ e : TNat → Γ ⊢ₜ e : TInt *)
+
+| Effect_typed Δ Γ1 e s ρ τ Γ2 :
+  let Abs_ρ := RCons (SAbs s) ρ in
+
+  vars._fresh s Γ1 ρ τ →
+  (<[ s := () ]> Δ) .| Γ1 ⊢ₜ e : Abs_ρ : τ ⊣ Γ2 →
+  Δ .| Γ1 ⊢ₜ Effect s e : ρ : τ ⊣ Γ2
+| Do_typed Δ Γ1 s e ρ' τ ι κ m Γ2 :
+  m m⪯C Γ2 →
+  Δ !! s = Some () →
+  let ρ := RCons (SFlip m (SSig s ι κ)) ρ' in
+  Δ .| Γ1 ⊢ₜ e : ρ : ι.[τ/] ⊣ Γ2 →
+                    Δ .| Γ1 ⊢ₜ Do (EffName s) e : ρ : κ.[τ/] ⊣ Γ2
+| DeepHandle_typed Δ Γ1 Γ2 Γ (m : mode) s e x k h y r ρ0 σ τ τ' ι κ :
+  le.MultiC Γ →
+  Δ !! s = Some () →
+  le.eff_name_from_sig σ = s →
+  let ρ := RCons σ ρ0 in
+  let ρ' := RCons (SFlip m (SSig s ι κ)) ρ0 in
+  Δ .| Γ1 ⊢ₜ e : ρ' : τ ⊣ Γ2 →
+  Δ .| <[ y :=c τ ]> (Γ2 ;; Γ) ⊢ₜ r : ρ : τ' ⊣ Γ →
+  Δ .| <[ x :=c ι ]> <[ k :=c ![m] (κ -{ ρ }-∘ τ') ]> Γ ⊢ₜ h : ρ : τ' ⊣ Γ →
+  Δ .| (Γ1 ;; Γ) ⊢ₜ (Handle Deep m s e (Lam x (Lam k h)) (Lam y r)) : ρ : τ' ⊣ Γ
+with val_typed : val → type → Prop :=
+| Unit_val_typed : ⊢ᵥ LitV LitUnit : ()
+where "Δ .| Γ1 ⊢ₜ e : ρ : τ ⊣ Γ2" := (typed Δ Γ1 e ρ τ Γ2)
+and "⊢ᵥ e : τ" := (val_typed e τ).                   
 
 
 
